

$ e^x=\sum_{n=0}^{\infty} \frac{x^n}{n !}=1+x+\frac{x^2}{2}+\frac{x^3}{6}+\cdots+\frac{x^n}{k !}+\cdots \\$

$ \ln (1+x)=\sum_{n=0}^{\infty} \frac{(-1)^n}{n+1} x^{n+1}=x-\frac{x^2}{2}+\frac{x^3}{3}-\frac{x^4}{4}+\cdots+\frac{(-1)^k x^{k+1}}{k+1}+\cdots, x \in(-1,1] \\$

$ \sin x=\sum_{n=0}^{\infty} \frac{(-1)^n}{(2 n+1) !} x^{2 n+1}=x-\frac{x^3}{6}+\frac{x^5}{120}-\cdots+\frac{(-1)^k}{(2 k+1) !} x^{2 k+1}+\cdots \\$

$ \cos x=\sum_{n=0}^{\infty} \frac{(-1)^n}{(2 n) !} x^{2 n}=1-\frac{x^2}{2}+\frac{x^4}{24}-\cdots+\frac{(-1)^k}{(2 k) !} x^{2 k}+\cdots \\$

$ \tan x=2 \sum_{n=1}^{\infty} \frac{\left(4^n-1\right) \zeta(2 n)}{\pi^{2 n}} x^{2 n-1}=x+\frac{1}{3} x^3+\frac{2}{15} x^5+\frac{17}{315} x^7+\frac{62}{2835} x^9+\frac{1382}{155925} x^{11}+o\left(x^{12}\right), x \in\left(-\frac{\pi}{2}, \frac{\pi}{2}\right) \\$

$ \sec x=\sum_{n=0}^{\infty} \frac{(-1)^n E_{2 n}}{(2 n) !} x_{2 n}=1+\frac{1}{2} x^2+\frac{5}{24} x^4+\frac{61}{720} x^6+\frac{277}{8064} x^8+\frac{50521}{3628800} x^{10}+o\left(x^{11}\right), x \in\left(-\frac{\pi}{2}, \frac{\pi}{2}\right) \\$

$ \arcsin x=\sum_{n=0}^{\infty} \frac{C_{2 n}^n}{4^n(2 n+1)} x^{2 n+1}=x+\frac{1}{6} x^3+\frac{3}{40} x^5+\frac{5}{112} x^7+\frac{35}{1152} x^9+\frac{63}{2816} x^{11}+o\left(x^{12}\right), x \in(-1,1) \\$

$ \arctan x=\sum_{n=0}^{\infty} \frac{(-1)^n}{2 n+1} x^{2 n+1}=x-\frac{1}{3} x^3+\frac{1}{5} x^5-\cdots+\frac{(-1)^k}{2 k+1} x^{2 k+1}+\cdots, x \in(-1,1) \\$

$ \sinh x=\sum_{n=0}^{\infty} \frac{x^{2 n+1}}{(2 n+1) !}=x+\frac{1}{6} x^3+\frac{1}{120} x^5+\cdots+\frac{x^{2 k+1}}{(2 k+1) !}+\cdots \\$

$ \cosh x=\sum_{n=0}^{\infty} \frac{x^{2 n}}{(2 n) !}=1+\frac{1}{2} x^2+\frac{1}{24} x^4+\cdots+\frac{x^{2 k}}{(2 k) !}+\cdots \\$

$ \tanh x=\sum_{n=1}^{\infty} \frac{4^n\left(4^n-1\right) B_{2 n}}{(2 n) !} x^{2 n-1}=x-\frac{1}{3} x^3+\frac{2}{15} x^5-\frac{17}{315} x^7+\frac{62}{2835} x^9-\frac{1382}{155925} x^{11}+o\left(x^{12}\right), x \in\left(-\frac{\pi}{2}, \frac{\pi}{2}\right) \\$

$ \operatorname{sech} x=\sum_{n=0}^{\infty} \frac{E_{2 n} x^{2 n}}{(2 n) !}=1-\frac{1}{2} x^2+\frac{5}{24} x^4-\frac{61}{720} x^6+\frac{277}{8064} x^8-\frac{50521}{3628800} x^{10}+o\left(x^{11}\right), x \in\left(-\frac{\pi}{2}, \frac{\pi}{2}\right) \\$

$ \operatorname{arsinh} x=\sum_{n=0}^{\infty} \frac{(-1)^n C_{2 n}^n}{4^n(2 n+1)} x^{2 n+1}=x-\frac{1}{6} x^3+\frac{3}{40} x^5-\frac{5}{112} x^7+\frac{35}{1152} x^9-\frac{63}{2816} x^{11}+o\left(x^{12}\right), x \in(-1,1) \\$

$ \operatorname{artanh} x=\sum_{n=0}^{\infty} \frac{x^{2 n+1}}{2 n+1}=x+\frac{1}{3} x^3+\frac{1}{5} x^5+\frac{1}{7} x^7+\frac{1}{9} x^9+\frac{1}{11} x^{11}+o\left(x^{12}\right), x \in(-1,1) \\$

$ e^{\mathrm{sin} z}=1+x+\frac{1}{2} x^2-\frac{1}{8} x^4-\frac{1}{15} x^5-\frac{1}{240} x^6+\frac{1}{90} x^7+\frac{31}{5760} x^8+\frac{1}{5670} x^9-\frac{2951}{3628800} x^{10}+o\left(x^{10}\right) \\$

$ e^{\tan x}=1+x+\frac{1}{2} x^2+\frac{1}{2} x^3+\frac{3}{8} x^4+\frac{37}{120} x^5+\frac{59}{240} x^6+\frac{137}{720} x^7+\frac{871}{5760} x^8+\frac{41641}{3628800} x^9+o\left(x^9\right) \\$

$ e^{\text {arrain } x}=1+x+\frac{1}{2} x^2+\frac{1}{3} x^3+\frac{5}{24} x^4+\frac{1}{6} x^5+\frac{17}{144} x^6+\frac{13}{126} x^7+\frac{629}{8064} x^8+\frac{325}{4536} x^9+o\left(x^9\right) \\$

$ e^{\arctan x}=1+x+\frac{1}{2} x^2-\frac{1}{6} x^3-\frac{7}{24} x^4+\frac{1}{24} x^5+\frac{29}{144} x^6-\frac{1}{1008} x^7-\frac{1219}{8064} x^8-\frac{1163}{72576} x^9+o\left(x^9\right) \\$

$ \tan (\tan x)=x+\frac{2}{3} x^3+\frac{3}{5} x^5+\frac{181}{315} x^7+\frac{59}{105} x^9+\frac{3455}{6237} x^{11}+o\left(x^{12}\right) \\$

$ \sin (\sin x)=x-\frac{1}{3} x^3+\frac{1}{10} x^5-\frac{8}{315} x^7+\frac{13}{2520} x^9-\frac{47}{49896} x^{11}+o\left(x^{12}\right) \\$

$ \tan (\sin x)=x+\frac{1}{6} x^3-\frac{1}{40} x^5-\frac{107}{5040} x^7-\frac{73}{24192} x^9+\frac{41897}{39916800} x^{11}+o\left(x^{12}\right) \\$

$ \sin (\tan x)=x+\frac{1}{6} x^3-\frac{1}{40} x^5-\frac{55}{1008} x^7-\frac{143}{3456} x^0-\frac{968167}{39916800} x^{11}+o\left(x^{12}\right) \\$

$ (1+x)^n=1+\sum_{n=1}^{\infty} \frac{\alpha(\alpha-1) \cdots(\alpha-n+1)}{n !} x^n=1+\alpha x+\frac{\alpha(\alpha-1)}{2 !} x^2+\cdots+\frac{\alpha(\alpha-1) \cdots(\alpha-k+1)}{k !} x^k+\cdots, x \in(-1,1) \\$

$ (1+x)^{\frac{1}{x}}=e-\frac{e}{2} x+\frac{11 e}{24} x^2-\frac{7 e}{16} x^3+\frac{2447 e}{5760} x^4-\frac{959 e}{2304} x^5+\frac{238043 e}{580608} x^6-\frac{67223 e}{165888} x^7+o\left(x^7\right) \\$

$ \left(1+x^2\right)^{\frac{1}{x}}=1+x+\frac{1}{2} x^2-\frac{1}{3} x^3-\frac{11}{24} x^4+\frac{11}{120} x^5+\frac{271}{720} x^6+\frac{53}{2520} x^7-\frac{4069}{13440} x^8+o\left(x^8\right) \\$

$(1+\sin x)^{\frac{1}{x}}=e-\frac{e}{2} x+\frac{7 e}{24} x^2-\frac{3 e}{16} x^3+\frac{139 e}{1152} x^4-\frac{899 e}{11520} x^5+\frac{29311 e}{580608} x^6-\frac{189617 e}{5806080} x^7+o\left(x^7\right) \\ $





 

vvc
